DelayedSystemF: hacks, still not working

devel/Iron/Language/DelayedSystemF/SubstTT.v
@@ -3,20 +3,24 @@ Require Export Iron.Language.DelayedSystemF.Ty.
 
 
 (* Apply an type substitution to a type. *)
-Fixpoint substTT (ss: @subst ty ki) (tt: ty) {struct tt} : ty  :=
+Fixpoint substTT (st: @subst ty ki) (tt: ty) {struct tt} : ty  :=
  match tt with
  |  TCon c
  => tt
 
  |  TVar a
- => match lookupSubst a ss with
+ => match lookupSubst a st with
     | None                => tt
     | Some (BBind _ _ t)  => t
     end
 
- |  TForall ss2 a k t
- => TForall (ss >< mapExpOfSubst (substTT ss) ss2) a k t
+ |  TForall st2 a k t
+ => TForall (st >< mapExpOfSubst (substTT st) st2) a k t
 
  |  TFun t1 t2
- => TFun (substTT ss t1) (substTT ss t2)
+ => TFun (substTT st t1) (substTT st t2)
  end.
+
+
+Definition substTE (st: @subst ty ki) (ee: @env ty): @env ty :=
+ map (mapTypeOfSig (substTT st)) ee.
