devel/Iron/Language/DelayedSystemF/SubstXX.v
@@ -3,36 +3,41 @@ Require Export Iron.Language.DelayedSystemF.TypeX.
 
 
 (* Apply an expression substitution to an expression. *)
-Fixpoint substXX (ss: @subst exp ty) (xx: exp) {struct xx} : exp  :=
+Fixpoint substXX (st: @subst ty ki) (sx: @subst exp ty) 
+                 (xx: exp) {struct xx} : exp  :=
  match xx with
- | XVar n
- => match lookupSubst n ss with
+ |  XVar n
+ => match lookupSubst n sx with
     | None                => xx
     | Some (BBind _ _ x)  => x
     end
 
- |  XAbs sx n t x
- => XAbs (ss >< mapExpOfSubst (substXX ss) sx) n t x
+ |  XAbs st2 sx2 n t x
+ => XAbs (st >< mapExpOfSubst (substTT st)    st2) 
+         (sx >< mapExpOfSubst (substXX st sx) sx2)
+          n t x
 
  |  XApp x1 x2
- => XApp (substXX ss x1) (substXX ss x2)
+ => XApp (substXX st sx x1)   (substXX st sx x2)
 
- |  XABS st sx a k x
- => XABS st (ss >< mapExpOfSubst (substXX ss) sx) a k x
+ |  XABS st2 sx2 a k x
+ => XABS (st >< mapExpOfSubst (substTT st)    st2)
+         (sx >< mapExpOfSubst (substXX st sx) sx2) 
+          a k x
 
  |  XAPP x1 t2 
- => XAPP (substXX ss x1) t2
+ => XAPP (substXX st sx x1) t2
  end.
 
 
 (* Substitution of expressions in expressions preserves typing. *)
 Lemma subst_exp_exp
- :  forall ke te sx x t
- ,  TypeX  ke (te >< stripS sx) x t
- -> ForallSubstXT (TypeX ke te) sx
- -> TypeX  ke te (substXX sx x) t.
+ :  forall ke te st sx x t
+ ,  TypeX  (ke >< stripS st) (te >< stripS sx) x t
+ -> ForallSubstXT (TypeX ke (substTE st te)) sx
+ -> TypeX  ke (substTE st te) (substXX st sx x) (substTT st t).
 Proof.
- intros. gen ke te sx t.
+ intros. gen ke te st sx t.
  induction x using exp_iind;
   intros; simpl in *.
 
@@ -62,13 +67,14 @@ Proof.
 
      eapply (Forall_inst ke)  in H.
      eapply (Forall_inst te)  in H.
+     eapply (Forall_inst st0) in H.
      eapply (Forall_inst sx0) in H.
      eapply (Forall_mp_const) in H; auto.
 
      eapply (Forall_map 
               (  fun xx => forall t
-              ,  TypeX ke (te >< stripS sx0) xx t
-              -> TypeX ke te (substXX sx0 xx) t)) in H.
+              ,  TypeX (ke >< stripS st0) (te >< stripS sx0) xx t
+              -> TypeX ke te (substXX st0 sx0 xx) t)) in H.
 
      eapply Forall_Forall2_right  in H.
      eapply ForallSubstXT_fold    in H.
@@ -77,9 +83,10 @@ Proof.
      eapply ForallSubstXT_mp; eauto.
 
    + unfold stripS.
-     rewrite map_app.
-     rewrite stripS_fold.
-     rewrite stripS_mapExpOfSubst.
+     repeat (rewrite map_app).
+     repeat (rewrite stripS_fold).
+     repeat (rewrite stripS_mapExpOfSubst).
+     rewrite <- app_assoc.
      rewrite <- app_assoc.
      assumption.
 
