devel/Iron/Language/DelayedSystemF/TypeX.v
@@ -12,10 +12,12 @@ Inductive TypeX : kienv -> tyenv -> exp -> ty -> Prop :=
    -> TypeX  ke te (XVar v) t
 
  | TxAbs
-   :  forall ke te sx v1 t1 x2 t2
+   :  forall ke te st sx v1 t1 x2 t2
    ,  ForallSubstXT (TypeX ke te) sx
-   -> TypeX  ke (te >< stripS sx :> SSig v1 t1) x2 t2
-   -> TypeX  ke te (XAbs sx v1 t1 x2) (TFun t1 t2)
+   -> TypeX  (ke >< stripS st)
+             (te >< stripS sx :> SSig v1 t1) 
+             x2 t2
+   -> TypeX  ke te (XAbs st sx v1 t1 x2) (TFun t1 t2)
 
  (* TODO need type equiv here, rather than just t1 *)
  | TxApp
@@ -24,9 +26,12 @@ Inductive TypeX : kienv -> tyenv -> exp -> ty -> Prop :=
    -> TypeX  ke te x2 t1
    -> TypeX  ke te (XApp x1 x2) t2
 
+ (* TODO need type equiv, don't require forall binder to have same name *)
  | TxABS
    :  forall ke te st sx a1 k1 x2 t2
-   ,  TypeX  (ke >< stripS st :> SSig a1 k1) (te >< stripS sx) x2 t2
+   ,  TypeX  (ke >< stripS st :> SSig a1 k1)
+             (te >< stripS sx)
+             x2 t2
    -> TypeX  ke te (XABS st sx a1 k1 x2) (TForall st a1 k1 t2)
 
  | TxAPP
@@ -42,7 +47,7 @@ Ltac inverts_type :=
  repeat 
   (match goal with 
    | [ H: TypeX _ _ (XVar _) _         |- _ ] => inverts H
-   | [ H: TypeX _ _ (XAbs _ _ _ _) _   |- _ ] => inverts H
+   | [ H: TypeX _ _ (XAbs _ _ _ _ _) _ |- _ ] => inverts H
    | [ H: TypeX _ _ (XApp _ _) _       |- _ ] => inverts H
    | [ H: TypeX _ _ (XABS _ _ _ _ _) _ |- _ ] => inverts H
    | [ H: TypeX _ _ (XAPP _ _) _       |- _ ] => inverts H
